theories/imp_to_asm_examples.v
@@ -93,19 +93,35 @@ Ltac simpl_map_ext tac ::=
          | |- context [ map_scramble ?ns ?m (<[?i:=?x]> ?m') ] =>
              is_closed_term ns;
              rewrite ->(map_scramble_insert_r_in ns m m' i x) by compute_done
+         | |- context [ map_preserved ?ns ?m (<[?i:=?x]> ?m') ] =>
+             is_closed_term ns;
+             rewrite ->(map_preserved_insert_r_not_in ns m m' i x) by compute_done
          | H : map_scramble ?ns (<[?i:=?x]> ?m) ?m' |- _ =>
              is_closed_term ns;
              rewrite ->(map_scramble_insert_l_in ns m m' i x) in H by compute_done
+         | H : map_preserved ?ns (<[?i:=?x]> ?m) ?m' |- _ =>
+             is_closed_term ns;
+             rewrite ->(map_preserved_insert_l_not_in ns m m' i x) in H by compute_done
          | H : map_scramble ?ns (<[?i:=?x]> ?m) ?m' |- _ =>
              is_closed_term ns;
              apply map_scramble_insert_l_not_in in H; [|compute_done];
              let H' := fresh in
              destruct H as [H' H]
+         | H : map_preserved ?ns (<[?i:=?x]> ?m) ?m' |- _ =>
+             is_closed_term ns;
+             apply map_preserved_insert_l_in in H; [|compute_done];
+             let H' := fresh in
+             destruct H as [H' H]
          | |- context [map_scramble ?ns ?m (<[?i:=?x]> ?m')] =>
              is_closed_term ns;
              rewrite ->(map_scramble_insert_r_not_in ns m m' i x) by compute_done
+         | |- context [map_preserved ?ns ?m (<[?i:=?x]> ?m')] =>
+             is_closed_term ns;
+             rewrite ->(map_preserved_insert_r_in ns m m' i x) by compute_done
          | |- context [ map_scramble ?ns ?m ?m ] =>
              rewrite ->(map_scramble_eq' ns m)
+         | |- context [ map_preserved ?ns ?m ?m ] =>
+             rewrite ->(map_preserved_eq' ns m)
          end.
 
 
@@ -124,8 +140,8 @@ Proof.
   tstep_i => ??. simplify_map_eq'.
   tstep_i; simplify_map_eq'. split!.
   go_s => n1 n2 ??; subst.
-  apply: Hret; [by simplify_map_eq| |done..].
-  unfold imp_to_asm_ret; split!; by simplify_map_eq'.
+  apply: Hret; [by simplify_map_eq| |done|done|by simplify_map_eq'|done].
+  unfold imp_to_asm_ret; split!; simplify_map_eq' => //.
 Qed.
 
 Lemma asm_add_client_refines_imp_add_client :
@@ -164,7 +180,7 @@ Proof.
   change (imp.Call "add" [Val 1; Val 1]) with (expr_fill [] (imp.Call "add" [Val 1; Val 1])).
   apply: Hcall. { repeat econs. } { by simplify_map_eq. } { set_solver. } { set_solver. } { by simplify_map_eq. }
   { unfold imp_to_asm_args. split!; decompose_Forall; by simplify_map_eq'. }
-  { by simplify_map_eq. } { done. } { done. }
+  { by simplify_map_eq. } { done. } { done. } { by simplify_map_eq'. }
   move => rs'' mem'' v h'' ? pb'' Hpc'' Hv Hmem ? ?.
   move: Hv => [?[? Hm]]; simplify_map_eq'.
   tstep_i; simplify_map_eq'. split!; [by simplify_map_eq'..|].
@@ -173,7 +189,7 @@ Proof.
   tstep_i => ??. simplify_map_eq'.
   have ->: rs !!! "SP" - 1 + 1 = rs !!! "SP" by lia.
   tstep_i; simplify_map_eq'. split; [done|].
-  apply: Hret; [| | |done|done]. { simplify_map_eq'. f_equal. etrans; [eapply Hmem|]; by simplify_map_eq'. }
+  apply: Hret; [| | |done|by simplify_map_eq'|done]. { simplify_map_eq'. f_equal. etrans; [eapply Hmem|]; by simplify_map_eq'. }
   2 : { move => ?. simplify_map_eq' => ?. etrans; [eapply Hmem; simplify_map_eq'; lia|].
         rewrite lookup_total_insert_ne //. lia. }
   unfold imp_to_asm_ret; split!; simplify_map_eq'; split!.
@@ -243,7 +259,6 @@ set_secret :
 
 The interesting property to prove here would be to prove that SECRET is 1 when calling ext
 and showing that this can be proven even if one refines c_code to Call "set_secret".
-The current imp_to_asm seems to enforce a condition that is too strong (almost all registers must
-be preserved between call and return)
-
+This requires exploiting the fact that imp_to_asm guarantees that the C code only touches
+certain registers.
 *)
